Refactor the full_spec tc proof

theories/examples/enclaves/trusted_compute.v
@@ -780,6 +780,133 @@ Section trusted_compute_example.
     iApply "Hcont"; iFrame.
   Admitted.
 
+  Definition tc_mainN := (trusted_computeN.@"main").
+  Definition tc_main_inv b_main e_main pc_v main_code a_data link_cap
+    := na_inv logrel_nais tc_mainN
+         (codefrag b_main pc_v main_code
+          ∗ (a_data, pc_v) ↦ₐ link_cap
+          ∗ ((a_data ^+ 1)%a, pc_v) ↦ₐ LCap RWX b_main e_main a_data pc_v).
+
+  Lemma trusted_compute_callback_code_sentry
+    (b_main : Addr)
+    (pc_v : Version)
+
+    (b_link a_link e_link assert_entry : Addr) (* linking *)
+    (assert_lt_offset : Z)
+    (b_assert e_assert a_flag : Addr) (v_assert : Version) (* assert *)
+    (tc_addr : Addr)
+    :
+
+    let v_link := pc_v in
+    let link_cap := LCap RO b_link e_link a_link v_link in
+
+    let e_main := (b_main ^+ trusted_compute_main_len)%a in
+    let a_callback := (b_main ^+ trusted_compute_main_init_len)%a in
+    let a_data := (b_main ^+ trusted_compute_main_code_len)%a in
+
+    let trusted_compute_main := trusted_compute_main_code assert_lt_offset in
+    ContiguousRegion b_main trusted_compute_main_len ->
+
+    (a_link + assert_lt_offset)%a = Some assert_entry →
+    withinBounds b_link e_link assert_entry = true ->
+    (link_table_inv
+       v_link
+       assert_entry b_assert e_assert v_assert
+     ∗ assert_inv b_assert a_flag e_assert v_assert
+     ∗ flag_inv a_flag v_assert
+     ∗ tc_main_inv b_main e_main pc_v (trusted_compute_main_code assert_lt_offset tc_addr) a_data link_cap
+    )
+    ∗ custom_enclave_inv (tcenclaves_map tc_addr)
+    ⊢ interp (LCap E b_main (b_main ^+ trusted_compute_main_len)%a
+                (b_main ^+ trusted_compute_main_init_len)%a pc_v).
+  Proof.
+    intros ?????? Hregion Hassert Hlink.
+    iIntros "[#(HlinkInv & HassertInv & HflagInv & HcodeInv) #Hcemap_inv]".
+    iEval (rewrite fixpoint_interp1_eq /=).
+    iIntros (regs); iNext ; iModIntro.
+    iIntros "( [%Hrmap_full #Hrmap_interp] & Hrmap & Hna)".
+    rewrite /registers_mapsto.
+    iExtract "Hrmap" PC as "HPC".
+    cbn in Hrmap_full.
+    destruct (Hrmap_full r_t0) as [w0 Hr0].
+    destruct (Hrmap_full r_t1) as [w1 Hr1].
+    destruct (Hrmap_full r_t2) as [w2 Hr2].
+    destruct (Hrmap_full r_t3) as [w3 Hr3].
+    destruct (Hrmap_full r_t4) as [w4 Hr4].
+    destruct (Hrmap_full r_t5) as [w5 Hr5].
+    iExtractList "Hrmap" [r_t0;r_t1;r_t2;r_t3;r_t4;r_t5]
+      as ["Hr0";"Hr1";"Hr2";"Hr3";"Hr4";"Hr5"].
+
+    iAssert (interp w0) as "Hinterp_w0".
+    { iApply "Hrmap_interp";eauto;done. }
+    iAssert (interp w1) as "Hinterp_w1".
+    { iApply "Hrmap_interp";eauto;done. }
+
+
+    rewrite /interp_conf.
+    iApply (wp_wand _ _ _
+              ( fun v =>
+                  ((⌜v = HaltedV⌝ →
+                    ∃ lregs : LReg, full_map lregs
+                                    ∧ registers_mapsto lregs
+                                    ∗ na_own logrel_nais ⊤)
+                   ∨ ⌜v = FailedV⌝
+                  )%I)
+             with "[-]").
+
+    - iMod (na_inv_acc with "HcodeInv Hna") as "[>(Hcode & Hdata & Hdata') [Hna Hcls] ]"
+      ;[solve_ndisj|solve_ndisj|].
+
+      iApply ( (trusted_compute_callback_code_spec (⊤ ∖ ↑tc_mainN))
+               with "[$HlinkInv $HassertInv $HflagInv $Hcemap_inv Hinterp_w0 Hinterp_w1]
+                 [$HPC $Hr0 $Hr1 $Hr2 $Hr3 $Hr4 $Hr5 $Hcode $Hdata $Hdata' $Hna Hcls Hrmap]")
+      ; eauto
+      ; try solve_ndisj
+      ; try iFrame "∗#".
+      iNext; iIntros "(Hcode & Hadata & Hadata' & HPC & Hr0 & Hr1 & Hr2 & Hr3 & Hr4 & Hr5 & Hna)".
+      iMod ("Hcls" with "[$Hcode $Hadata $Hadata' $Hna]") as "Hna".
+      wp_end. iIntros (_).
+
+      (* Cannot use iInsert, because Qed is too long *)
+      iDestruct (big_sepM_insert _ _ r_t5 with "[$Hrmap $Hr5]") as "Hrmap"
+      ; first (by rewrite lookup_delete).
+      rewrite insert_delete_insert; repeat (rewrite -delete_insert_ne //=).
+      iDestruct (big_sepM_insert _ _ r_t4 with "[$Hrmap $Hr4]") as "Hrmap"
+      ; first (by rewrite lookup_delete).
+      rewrite insert_delete_insert; repeat (rewrite -delete_insert_ne //=).
+      iDestruct (big_sepM_insert _ _ r_t3 with "[$Hrmap $Hr3]") as "Hrmap"
+      ; first (by rewrite lookup_delete).
+      rewrite insert_delete_insert; repeat (rewrite -delete_insert_ne //=).
+      iDestruct (big_sepM_insert _ _ r_t2 with "[$Hrmap $Hr2]") as "Hrmap"
+      ; first (by rewrite lookup_delete).
+      rewrite insert_delete_insert; repeat (rewrite -delete_insert_ne //=).
+      iDestruct (big_sepM_insert _ _ r_t1 with "[$Hrmap $Hr1]") as "Hrmap"
+      ; first (by rewrite lookup_delete).
+      rewrite insert_delete_insert; repeat (rewrite -delete_insert_ne //=).
+      iDestruct (big_sepM_insert _ _ r_t0 with "[$Hrmap $Hr0]") as "Hrmap"
+      ; first (by rewrite lookup_delete).
+      rewrite insert_delete_insert; repeat (rewrite -delete_insert_ne //=).
+      iDestruct (big_sepM_insert _ _ PC with "[$Hrmap $HPC]") as "Hrmap"
+      ; first (by rewrite lookup_delete).
+      rewrite insert_delete_insert; repeat (rewrite -delete_insert_ne //=).
+      iExists _.
+      iFrame "∗".
+
+
+      iPureIntro; intros r; cbn.
+      destruct (decide (r=PC)); simplify_map_eq;first done.
+      destruct (decide (r=r_t5)); simplify_map_eq;first done.
+      destruct (decide (r=r_t4)); simplify_map_eq;first done.
+      destruct (decide (r=r_t3)); simplify_map_eq;first done.
+      destruct (decide (r=r_t2)); simplify_map_eq;first done.
+      destruct (decide (r=r_t1)); simplify_map_eq;first done.
+      destruct (decide (r=r_t0)); simplify_map_eq;first done.
+      apply Hrmap_full.
+    - iEval (cbn). iIntros (v) "H ->".
+      iDestruct "H" as "[H|%]"; last congruence.
+      by iApply "H".
+  Qed.
+
   Lemma trusted_compute_full_run_spec
     (b_main : Addr)
     (pc_v : Version)
@@ -813,12 +940,13 @@ Section trusted_compute_example.
        v_link
        assert_entry b_assert e_assert v_assert
     ∗ assert_inv b_assert a_flag e_assert v_assert
-    ∗ flag_inv a_flag v_assert)
+    ∗ flag_inv a_flag v_assert
+    ∗ tc_main_inv b_main e_main pc_v (trusted_compute_main_code assert_lt_offset tc_addr) a_data link_cap
+    )
     ∗ custom_enclave_inv (tcenclaves_map tc_addr)
     ∗ interp wadv
 
-    ⊢ ( codefrag b_main pc_v (trusted_compute_main tc_addr)
-        ∗ ((a_data)%a, pc_v) ↦ₐ link_cap
+    ⊢ ( ((a_data)%a, pc_v) ↦ₐ link_cap
         ∗ ((a_data ^+ 1)%a, pc_v) ↦ₐ (LCap RWX b_main e_main a_data pc_v)
 
           ∗ PC ↦ᵣ LCap RWX b_main e_main b_main pc_v
@@ -832,13 +960,15 @@ Section trusted_compute_example.
   Proof.
     intros ?????? Hregion Hassert Hlink Hrmap.
 
-    iIntros "#[ [HlinkInv [HassertInv HflagInv] ] [ Hcemap_inv Hinterp_wadv ] ]
-             (Hcode & Hadata & Hadata' & HPC & Hr0 & Hr1 & Hrmap & Hna)".
+    iIntros "[  #(HlinkInv & HassertInv & HflagInv & HcodeInv) #[ Hcemap_inv Hinterp_wadv ] ]
+             (Hadata & Hadata' & HPC & Hr0 & Hr1 & Hrmap & Hna)".
 
     iDestruct (jmp_to_unknown with "Hinterp_wadv") as "Hjmp".
-
+    iMod (na_inv_acc with "HcodeInv Hna") as "[>(Hcode & Hdata & Hdata') [Hna Hcls] ]"
+    ;[solve_ndisj|solve_ndisj|].
     iApply (trusted_compute_main_init_spec with "[-]"); eauto; iFrame.
     iNext; iIntros "(Hcode & HPC & Hr0 & Hr1)".
+    iMod ("Hcls" with "[$Hcode $Hadata $Hadata' $Hna]") as "Hna".
 
     (* Show that the contents of unused registers is safe *)
     iAssert ([∗ map] r↦w ∈ rmap, r ↦ᵣ w ∗ interp w)%I with "[Hrmap]" as "Hrmap".
@@ -848,125 +978,22 @@ Section trusted_compute_example.
     }
 
     (* Show the content of r1 is safe *)
-    iMod (na_inv_alloc logrel_nais _ (trusted_computeN.@"code")
-            (codefrag b_main pc_v (trusted_compute_main_code assert_lt_offset tc_addr)
-             ∗ (a_data, pc_v) ↦ₐ link_cap
-             ∗ ((a_data ^+ 1)%a, pc_v) ↦ₐ LCap RWX b_main e_main a_data pc_v
-            )%I
-           with "[$Hcode $Hadata $Hadata']")
-      as "#Hcode".
-
-    set ( wret :=
-        LCap E b_main (b_main ^+ trusted_compute_main_len)%a
-               (b_main ^+ trusted_compute_main_init_len)%a pc_v).
-    iAssert (interp wret) as "Hinterp_ret".
-    {
-      iEval (rewrite fixpoint_interp1_eq /=).
-      iIntros (regs); iNext ; iModIntro.
-      iIntros "( [%Hrmap_full #Hrmap_interp] & Hrmap & Hna)".
-      rewrite /registers_mapsto.
-      iExtract "Hrmap" PC as "HPC".
-      cbn in Hrmap_full.
-      destruct (Hrmap_full r_t0) as [w0 Hr0].
-      clear w1; destruct (Hrmap_full r_t1) as [w1 Hr1].
-      destruct (Hrmap_full r_t2) as [w2 Hr2].
-      destruct (Hrmap_full r_t3) as [w3 Hr3].
-      destruct (Hrmap_full r_t4) as [w4 Hr4].
-      destruct (Hrmap_full r_t5) as [w5 Hr5].
-      iExtractList "Hrmap" [r_t0;r_t1;r_t2;r_t3;r_t4;r_t5]
-        as ["Hr0";"Hr1";"Hr2";"Hr3";"Hr4";"Hr5"].
-
-      rewrite /interp_conf.
-      iApply (wp_wand _ _ _
-                ( fun v =>
-                    ((⌜v = HaltedV⌝ →
-                     ∃ lregs : LReg, full_map lregs
-                                     ∧ registers_mapsto lregs
-                                     ∗ na_own logrel_nais ⊤)
-                      ∨ ⌜v = FailedV⌝
-                    )%I)
-               with "[-]").
-
-      - iAssert (interp w0) as "Hinterp_w0".
-        { iApply "Hrmap_interp";eauto;done. }
-        iAssert (interp w1) as "Hinterp_w1".
-        { iApply "Hrmap_interp";eauto;done. }
-
-        iMod (na_inv_acc with "Hcode Hna") as "[>(Hcode' & Hdata & Hdata') [Hna Hcls] ]"
-        ;[solve_ndisj|solve_ndisj|].
-        set (E := (⊤ ∖ ↑trusted_computeN.@"code")).
-        iApply ( (trusted_compute_callback_code_spec E)
-                 with "[$HlinkInv $HassertInv $HflagInv $Hcemap_inv Hinterp_w0 Hinterp_w1]
-                 [$HPC $Hr0 $Hr1 $Hr2 $Hr3 $Hr4 $Hr5 $Hcode' $Hdata $Hdata' $Hna Hcls Hrmap]")
-        ; eauto
-        ; try solve_ndisj
-        ; try iFrame "∗#".
-        iNext; iIntros "(Hcode' & Hadata & Hadata' & HPC & Hr0 & Hr1 & Hr2 & Hr3 & Hr4 & Hr5 & Hna)".
-        iMod ("Hcls" with "[$Hcode' $Hadata $Hadata' $Hna]") as "Hna".
-        wp_end. iIntros (_).
-
-        (* Cannot use iInsert, because Qed is too long *)
-        iDestruct (big_sepM_insert _ _ r_t5 with "[$Hrmap $Hr5]") as "Hrmap"
-        ; first (by rewrite lookup_delete).
-        rewrite insert_delete_insert; repeat (rewrite -delete_insert_ne //=).
-        iDestruct (big_sepM_insert _ _ r_t4 with "[$Hrmap $Hr4]") as "Hrmap"
-        ; first (by rewrite lookup_delete).
-        rewrite insert_delete_insert; repeat (rewrite -delete_insert_ne //=).
-        iDestruct (big_sepM_insert _ _ r_t3 with "[$Hrmap $Hr3]") as "Hrmap"
-        ; first (by rewrite lookup_delete).
-        rewrite insert_delete_insert; repeat (rewrite -delete_insert_ne //=).
-        iDestruct (big_sepM_insert _ _ r_t2 with "[$Hrmap $Hr2]") as "Hrmap"
-        ; first (by rewrite lookup_delete).
-        rewrite insert_delete_insert; repeat (rewrite -delete_insert_ne //=).
-        iDestruct (big_sepM_insert _ _ r_t1 with "[$Hrmap $Hr1]") as "Hrmap"
-        ; first (by rewrite lookup_delete).
-        rewrite insert_delete_insert; repeat (rewrite -delete_insert_ne //=).
-        iDestruct (big_sepM_insert _ _ r_t0 with "[$Hrmap $Hr0]") as "Hrmap"
-        ; first (by rewrite lookup_delete).
-        rewrite insert_delete_insert; repeat (rewrite -delete_insert_ne //=).
-        iDestruct (big_sepM_insert _ _ PC with "[$Hrmap $HPC]") as "Hrmap"
-        ; first (by rewrite lookup_delete).
-        rewrite insert_delete_insert; repeat (rewrite -delete_insert_ne //=).
-        iExists _.
-        iFrame "∗".
-
-
-        iPureIntro; intros r; cbn.
-        destruct (decide (r=PC)); simplify_map_eq;first done.
-        destruct (decide (r=r_t5)); simplify_map_eq;first done.
-        destruct (decide (r=r_t4)); simplify_map_eq;first done.
-        destruct (decide (r=r_t3)); simplify_map_eq;first done.
-        destruct (decide (r=r_t2)); simplify_map_eq;first done.
-        destruct (decide (r=r_t1)); simplify_map_eq;first done.
-        destruct (decide (r=r_t0)); simplify_map_eq;first done.
-        apply Hrmap_full.
-      - iEval (cbn). iIntros (v) "H ->".
-        iDestruct "H" as "[H|%]"; last congruence.
-        by iApply "H".
-    }
+    iDestruct (trusted_compute_callback_code_sentry
+                with "[$HlinkInv $HassertInv $HflagInv $HcodeInv $Hcemap_inv]")
+      as "Hinterp_wret"; eauto.
+    (* Cannot use iInsert, because Qed is too long *)
+    iDestruct (big_sepM_insert _ _ r_t1 with "[$Hrmap $Hr1 $Hinterp_wret]") as "Hrmap"
+    ; first (apply not_elem_of_dom_1; rewrite Hrmap; set_solver).
+    iDestruct (big_sepM_insert _ _ r_t0 with "[$Hrmap $Hr0 $Hinterp_wadv]") as "Hrmap"
+    ; first (rewrite lookup_insert_ne //=; apply not_elem_of_dom_1; rewrite Hrmap; set_solver).
 
     (* Apply the result of the FTLR *)
-    iApply (wp_wand _ _ _
-              (λ v0 : val, ⌜v0 = HaltedV⌝ →
-                           ∃ lr : LReg, full_map lr
-                                        ∧ registers_mapsto lr
-                                        ∗ na_own logrel_nais ⊤)%I
-             with "[-]").
-    - iAssert (r_t0  ↦ᵣ wadv ∗ interp wadv)%I with "[$Hr0 $Hinterp_wadv]" as "Hr0".
-      iAssert (r_t1  ↦ᵣ wret ∗ interp wret)%I with "[$Hr1 $Hinterp_ret]" as "Hr1".
-
-      (* Cannot use iInsert, because Qed is too long *)
-      iDestruct (big_sepM_insert _ _ r_t1 with "[$Hrmap $Hr1]") as "Hrmap"
-      ; first (apply not_elem_of_dom_1; rewrite Hrmap; set_solver).
-      iDestruct (big_sepM_insert _ _ r_t0 with "[$Hrmap $Hr0]") as "Hrmap"
-      ; first (rewrite lookup_insert_ne //=; apply not_elem_of_dom_1; rewrite Hrmap; set_solver).
-      iApply ("Hjmp" with "[] [$HPC $Hrmap $Hna]") ;eauto.
-      iPureIntro.
-      rewrite !dom_insert_L Hrmap; set_solver.
-    - iIntros (v) "H". by iLeft.
+    iApply (wp_wand with "[-]").
+    - iApply ("Hjmp" with "[] [$HPC $Hrmap $Hna]") ;eauto.
+      iPureIntro; rewrite !dom_insert_L Hrmap; set_solver.
+    - iIntros (v) "H"; by iLeft.
   Qed.
 
-
-
+(* TODO @June adequacy theorem *)
 
 End trusted_compute_example.
